\section{Compilation}
First we translate the types:
$$\tau::=\ast\mid \obj\mid \tau\to\tau$$

$$\frac{\Gamma\vdash\alpha\Rightarrow \alpha'\quad \Gamma,x:\alpha\vdash \beta\Rightarrow \beta'}
{\Gamma\vdash\forall x:\alpha.\;\beta\Rightarrow
\begin{cases}
\ast&\mbox{if }\beta'=\ast\\
\alpha'\to\beta'&o.w.
\end{cases}}\qquad
\frac{}{\Gamma\vdash\U_\ell\Rightarrow \ast}\qquad
\frac{\Gamma\vdash\alpha\rightsquigarrow \alpha'\quad \Gamma\vdash \alpha'\Rightarrow \tau}
{\Gamma\vdash\alpha\Rightarrow\tau}$$
$$\frac{}{\Gamma\vdash(\mu t:(\forall x::\alpha.\;\P).\;K)\;e\Rightarrow \ast}\qquad
\frac{\ell\not\equiv 0}{\Gamma\vdash(\mu t:(\forall x::\alpha.\;\U_\ell).\;K)\;e\Rightarrow \obj}$$

Next we translate expressions:
$$e::=x\mid $$
$$\frac{}{\Gamma\vdash x\Rightarrow x}\qquad
\frac{}{\Gamma\vdash\U_\ell\Rightarrow \ast}\qquad
\frac{}{\Gamma\vdash\forall x:\alpha.\;\beta\Rightarrow \ast}$$
$$\qquad
\frac{\ell\not\equiv 0}{\Gamma\vdash(\mu t:(\forall x::\alpha.\;\U_\ell).\;K)\;e\Rightarrow \obj}$$

UNFINISHED
